finish refinement of conflict analysis to code

Weidenbach_Book/IsaSAT_Conflict_Analysis.thy
@@ -266,6 +266,7 @@ where
       let L' = atm_of L;
       ASSERT(arena_length N C \<noteq> 2 \<longrightarrow>
         curry6 isa_set_lookup_conflict_aa_pre M N C (b, (n, xs)) clvls lbd outl);
+      ASSERT(arena_is_valid_clause_idx N C);
       ((b, (n, xs)), clvls, lbd, outl) \<leftarrow>
         if arena_length N C = 2 then isasat_lookup_merge_eq2 L M N C (b, (n, xs)) clvls lbd outl
         else isa_resolve_merge_conflict_gt2 M N C (b, (n, xs)) clvls lbd outl;
@@ -303,7 +304,8 @@ definition update_confl_tl_wl_pre where
       distinct_mset (the (get_conflict_wl S)) \<and>
       - L \<notin> set (get_clauses_wl S \<propto> C) \<and>
       (length (get_clauses_wl S \<propto> C) > 2 \<longrightarrow> 
-        L \<notin> set (tl (get_clauses_wl S \<propto> C))) \<and>
+        L \<notin> set (tl (get_clauses_wl S \<propto> C)) \<and> 
+        get_clauses_wl S \<propto> C ! 0 = L) \<and>
       L \<in> set (watched_l (get_clauses_wl S \<propto> C)) \<and>
       distinct (get_clauses_wl S \<propto> C) \<and>
       \<not>tautology (the (get_conflict_wl S)) \<and>
@@ -345,8 +347,8 @@ lemma update_confl_tl_wl_heur_update_confl_tl_wl:
   [update_confl_tl_wl_pre]\<^sub>f
    nat_rel \<times>\<^sub>f Id \<times>\<^sub>f twl_st_heur_conflict_ana' r \<rightarrow> \<langle>bool_rel \<times>\<^sub>f twl_st_heur_conflict_ana' r\<rangle>nres_rel\<close>
 proof -
-(*
-  have H: \<open>isa_resolve_merge_conflict ba c a (aa, ab, bb) i k ag
+
+  have H: \<open>isa_resolve_merge_conflict_gt2 ba c a (aa, ab, bb) i k ag
         \<le> SPEC
           (\<lambda>x. (case x of
                 (x, xa) \<Rightarrow>
@@ -376,11 +378,19 @@ proof -
       \<in> nat_rel \<times>\<^sub>f nat_lit_lit_rel \<times>\<^sub>f twl_st_heur_conflict_ana' r\<close> and
       CLS[simp]: \<open>CLS = ((ao, bg), baa, ca, da, ea, fa, ga, ha)\<close> and
       \<open>CLS' = ((a, b), ba, c, (aa, ab, bb), e, f, ivmtf, h, i, j, k,
-        ag, (ah, ai, aj, be), ak, al, am, an, bf)\<close>
+        ag, (ah, ai, aj, be), ak, al, am, an, bf)\<close> and
+      le2: \<open>arena_length c a \<noteq> 2\<close>
     for a b ba c aa ab bb e f ac ad ae af bc bd h i j k ag ah ai aj be ak al am an
        bf ao bg baa ca da ea fa ga ha CLS CLS' ivmtf
   proof -
     let ?\<A> = \<open>all_atms_st (baa, ca, da, ea, fa, ga, ha)\<close>
+    have le2: \<open>length (ca \<propto> ao) > 2\<close>
+      using arena_lifting(19)[of c ca \<open>set an\<close> ao]
+      using rel inv le2 unfolding CLS update_confl_tl_wl_pre_def prod.case
+        get_clauses_wl.simps
+      by (auto simp: twl_st_heur_conflict_ana_def arena_lifting
+        simp del: arena_lifting(19))
+
     have
       ao: \<open>ao \<in># dom_m (get_clauses_wl (baa, ca, da, ea, fa, ga, ha))\<close> and
       conf: \<open>get_conflict_wl (baa, ca, da, ea, fa, ga, ha) \<noteq> None\<close> and
@@ -395,20 +405,21 @@ proof -
             (the (get_conflict_wl (baa, ca, da, ea, fa, ga, ha)))\<close> and
       dist_D: \<open>distinct_mset (the (get_conflict_wl (baa, ca, da, ea, fa, ga, ha)))\<close> and
       uL_NC: \<open>- bg \<notin> set (get_clauses_wl (baa, ca, da, ea, fa, ga, ha) \<propto> ao)\<close> and
-      L_NC: \<open>length (get_clauses_wl (baa, ca, da, ea, fa, ga, ha) \<propto> ao) > 2 \<longrightarrow>
-          bg \<notin> set (tl (get_clauses_wl (baa, ca, da, ea, fa, ga, ha) \<propto> ao))\<close> and
+      L_NC: \<open>bg \<notin> set (tl (get_clauses_wl (baa, ca, da, ea, fa, ga, ha) \<propto> ao))\<close> and
+      bg_hd: \<open>ca \<propto> ao ! 0 = bg\<close> and
       dist_NC: \<open>distinct (get_clauses_wl (baa, ca, da, ea, fa, ga, ha) \<propto> ao)\<close> and
       tauto_D:  \<open>\<not> tautology (the (get_conflict_wl (baa, ca, da, ea, fa, ga, ha)))\<close> and
       tauto_NC: \<open>\<not> tautology (mset (get_clauses_wl (baa, ca, da, ea, fa, ga, ha) \<propto> ao))\<close> and
       tauto_NC_D: \<open>\<not> tautology
-          (remove1_mset (- bg)
+          (remove1_mset bg (remove1_mset (- bg)
             (the (get_conflict_wl (baa, ca, da, ea, fa, ga, ha)) \<union>#
-            mset (tl (get_clauses_wl (baa, ca, da, ea, fa, ga, ha) \<propto> ao))))\<close> and
+            mset (get_clauses_wl (baa, ca, da, ea, fa, ga, ha) \<propto> ao))))\<close> and
       count_dec_ge: \<open>0 < count_decided (get_trail_wl (baa, ca, da, ea, fa, ga, ha))\<close> and
       lits_confl: \<open>literals_are_in_\<L>\<^sub>i\<^sub>n ?\<A> (the (get_conflict_wl (baa, ca, da, ea, fa, ga, ha)))\<close> and
       lits: \<open>literals_are_\<L>\<^sub>i\<^sub>n ?\<A> (baa, ca, da, ea, fa, ga, ha)\<close> and
       lits_trail: \<open>literals_are_in_\<L>\<^sub>i\<^sub>n_trail ?\<A> (get_trail_wl (baa, ca, da, ea, fa, ga, ha))\<close>
-      using inv unfolding CLS update_confl_tl_wl_pre_def prod.case
+      using inv le2 unfolding CLS update_confl_tl_wl_pre_def prod.case
+        get_clauses_wl.simps
       by blast+
     have
       n_d: \<open>no_dup baa\<close> and
@@ -438,20 +449,21 @@ proof -
       by (cases baa)
         (auto simp del: \<open>lit_of (hd baa) = bg\<close> simp: literals_are_in_\<L>\<^sub>i\<^sub>n_trail_Cons)
 
-    have [simp]: \<open>length (ca \<propto> ao) > 2 \<Longrightarrow> bg \<notin> set (tl (ca \<propto> ao))\<close>
+    have [simp]: \<open>bg \<notin> set (tl (ca \<propto> ao))\<close>
       using L_NC
       by (auto simp: resolve_cls_wl'_def split: if_splits)
     have mset_ge0_iff:  "0 < size M \<longleftrightarrow> M \<noteq> {#}" for M
      by (cases M) auto
-    have no_dup: \<open>length (ca \<propto> ao) > 2 \<Longrightarrow> L \<in> set (tl (ca \<propto> ao)) \<Longrightarrow> - L \<in># the da \<Longrightarrow> False\<close> for L
-      using tauto_NC_D tauto_NC \<open>length (ca \<propto> ao) > 2 \<Longrightarrow> bg \<notin> set (tl (ca \<propto> ao))\<close>
-      apply (cases \<open>- L \<in># mset (tl (ca \<propto> ao))\<close>; cases \<open>bg = L\<close>)
-      apply (auto dest!: multi_member_split
-      simp: sup_union_left2 add_mset_remove_trivial_If tautology_add_mset split: if_splits)
-      apply (metis in_set_tlD set_mset_mset tautology_minus)
-      by (metis \<open>bg \<notin># the da\<close> in_remove1_mset_neq insert_DiffM set_mset_mset
-        subset_mset.sup.right_idem subset_mset.sup_commute sup_union_left1 uminus_of_uminus_id
-        union_single_eq_member)
+    have no_dup: \<open>L \<in> set (tl (ca \<propto> ao)) \<Longrightarrow> - L \<in># the da \<Longrightarrow> False\<close> for L
+      using tauto_NC_D tauto_NC \<open>bg \<notin> set (tl (ca \<propto> ao))\<close> bg_hd le2
+      by (cases \<open>- L \<in># mset (tl (ca \<propto> ao))\<close>; cases \<open>bg = L\<close>; cases \<open>ca \<propto> ao\<close>)
+        (auto dest!: multi_member_split
+        simp: sup_union_left2 add_mset_remove_trivial_If
+          tautology_add_mset add_mset_eq_add_mset
+          add_mset_remove_trivial_eq  remove1_mset_union_distrib
+	dest: in_set_tlD tautology_minus[of L]
+        split: if_splits)
+
     have size_union_ge1: \<open>Suc 0 \<le> size A \<Longrightarrow> Suc 0 \<le> size (A \<union># B)\<close> for A B
       apply (cases A)
       apply (simp; fail)
@@ -494,7 +506,39 @@ proof -
     ultimately have [simp]: \<open>- bg \<notin># remove1_mset (- bg) (the da \<union># mset (tl (ca \<propto> ao)))\<close>
       by (metis \<open>a = ao\<close> diff_single_trivial in_multiset_in_set multi_drop_mem_not_eq
             remove1_mset_union_distrib)
+    have [simp]: \<open>bg \<notin># the da \<union># mset (ca \<propto> ao) - {#bg, - bg#}\<close>
+       \<open>-bg \<notin># the da \<union># mset (ca \<propto> ao) - {#bg, - bg#}\<close>
+      unfolding resolve_cls_wl'_def lookup_clause_rel_def
+        lookup_conflict_remove1_def
+      using dist_NC bg_hd le2
+	dist_NC[unfolded distinct_mset_mset_distinct[symmetric]]
+	multi_member_split[of \<open>bg\<close> \<open>mset (ca \<propto> ao)\<close>] tauto_NC_D
+	tauto_NC tauto_D uL_D dist_D
+     apply (cases \<open>bg \<in># the da\<close>)
+      apply (auto simp del: distinct_mset_mset_distinct
+        simp: tautology_add_mset sup_union_left2 sup_union_left1
+	  add_mset_eq_add_mset
+        dest!: in_set_takeD multi_member_split)
+       apply (metis distinct_mset_add_mset distinct_mset_union_mset
+         sup_union_right1 union_single_eq_member)
+       by (smt \<open>distinct_mset (mset (get_clauses_wl (baa, ca, da, ea, fa, ga, ha) \<propto> ao))\<close>
+	 add_mset_commute add_mset_diff_bothsides add_mset_remove_trivial_eq dist_D
+	 distinct_mset_add_mset distinct_mset_union_mset get_clauses_wl.simps
+	 get_conflict_wl.simps minus_notin_trivial2 remove_1_mset_id_iff_notin) 
 
+    have eq: \<open>(the da \<union># mset (ca \<propto> ao) - {#- bg, bg#}) =
+      remove1_mset (-bg) (the da \<union># mset (tl (ca \<propto> ao)))\<close>
+      unfolding resolve_cls_wl'_def lookup_clause_rel_def
+        lookup_conflict_remove1_def
+      using dist_NC bg_hd le2
+	dist_NC[unfolded distinct_mset_mset_distinct[symmetric]]
+	multi_member_split[of \<open>bg\<close> \<open>mset (ca \<propto> ao)\<close>] tauto_NC_D
+	tauto_NC tauto_D uL_D dist_D
+     by (cases \<open>ca \<propto> ao\<close>)
+      (auto simp del: distinct_mset_mset_distinct
+        simp: tautology_add_mset sup_union_left2 sup_union_left1
+	  add_mset_eq_add_mset
+        dest!: in_set_takeD multi_member_split)
     have \<open>vmtf_unset_pre (atm_of b) ivmtf\<close>
       if \<open>ivmtf \<in> isa_vmtf ?\<A> baa\<close>
       apply (rule vmtf_unset_pre'[OF that])
@@ -515,8 +559,9 @@ proof -
         by (cases baa; cases \<open>hd baa\<close>) auto
       then have out:
         \<open>out_learned baa (Some (resolve_cls_wl' (baa, ca, Some (the da), ea, fa, ga, ha) ao bg)) b\<close>
-        using uL_D H
-        by (auto simp: resolve_cls_wl'_def out_learned_def ac_simps)
+        using uL_D H bg_hd
+	by (cases \<open>ca \<propto> ao\<close>)
+          (auto simp: resolve_cls_wl'_def out_learned_def ac_simps)
       have \<open>out_learned (tl baa)
         (Some (resolve_cls_wl' (baa, ca, Some (the da), ea, fa, ga, ha) ao bg)) b\<close>
         apply (rule out_learned_tl_Some_notin[THEN iffD1])
@@ -525,7 +570,7 @@ proof -
     then show ?thesis
       using rel
       by (auto simp: twl_st_heur_conflict_ana_def merge_conflict_m_def update_confl_tl_wl_pre_def
-          resolve_cls_wl'_def ac_simps)
+          resolve_cls_wl'_def ac_simps eq)
     qed
     moreover have \<open>card_max_lvl baa (mset (tl (ca \<propto> ao)) \<union># (the da)) - Suc 0
       \<in> counts_maximum_level (tl baa)
@@ -534,7 +579,7 @@ proof -
       have \<open>distinct_mset (remove1_mset (- bg) (the da \<union># mset (tl (ca \<propto> ao))))\<close>
         using dist_NC dist_D by (auto intro!: distinct_mset_minus)
       moreover have \<open>\<not>tautology (remove1_mset (- bg) (the da \<union># mset (tl (ca \<propto> ao))))\<close>
-        using tauto_NC_D by simp
+        using tauto_NC_D by (simp add: eq[symmetric] ac_simps)
       moreover have \<open>card_max_lvl baa (mset (tl (ca \<propto> ao)) \<union># the da) - 1 =
         card_max_lvl baa (remove1_mset (- bg) (the da \<union># mset (tl (ca \<propto> ao))))\<close>
         unfolding \<open>lit_of (hd baa) = bg\<close> [symmetric]
@@ -544,7 +589,9 @@ proof -
       ultimately show ?thesis
         unfolding counts_maximum_level_def
         using uL_D L_M proped nempty \<open>ao > 0\<close> n_d count_dec_ge
-        by (auto simp del: simp: card_max_lvl_tl resolve_cls_wl'_def card_max_lvl_remove1_mset_hd)
+	unfolding eq
+        by (auto simp del: simp:ac_simps eq
+	  card_max_lvl_tl resolve_cls_wl'_def card_max_lvl_remove1_mset_hd)
     qed
     moreover have \<open>da = Some y \<Longrightarrow> ((a, aaa, b), Some (y \<union># mset (tl (ca \<propto> ao))))
        \<in> option_lookup_clause_rel ?\<A> \<Longrightarrow>
@@ -574,349 +621,17 @@ proof -
        using rel inv
        apply -
        apply (rule order_trans)
-       apply (rule isa_resolve_merge_conflict[of ?\<A> \<open>set an\<close>,
+       apply (rule isa_resolve_merge_conflict_gt2[of ?\<A> \<open>set an\<close>,
          THEN fref_to_Down_curry6, OF merge_conflict_m_pre])
        subgoal using arena ocr trail by (auto simp: all_atms_def[symmetric])
        subgoal unfolding merge_conflict_m_def conc_fun_SPEC
         by (auto simp: twl_st_heur_conflict_ana_def merge_conflict_m_def update_confl_tl_wl_pre_def
            resolve_cls_wl'_def ac_simps no_dup_tlD lookup_remove1_uminus arena_in_L
-	   all_atms_def[symmetric]
+	   all_atms_def[symmetric] eq
            intro!: ASSERT_refine_left
 	     tl_trail_tr[THEN fref_to_Down_unRET])
        done
   qed
-
-  have \<open>isa_resolve_merge_conflict (aa, ab, ac, ad, ae, ba) c a (af, x1, x2) i k l
-	\<le> SPEC
-	   (\<lambda>x. (case x of
-		 (x, xa) \<Rightarrow>
-		   (case x of
-		    (bb, n, xs) \<Rightarrow>
-		      \<lambda>(clvls, lbd, outl). do {
-			   _ \<leftarrow> ASSERT
-				(curry lookup_conflict_remove1_pre b (n, xs) \<and>
-				 1 \<le> clvls);
-			   let (n, xs) = lookup_conflict_remove1 b (n, xs);
-			   _ \<leftarrow> ASSERT
-				(vmtf_unset_pre (atm_of b)
-				  ((ah, ai, aj, ak, bc), al, bd));
-			   _ \<leftarrow> ASSERT (tl_trailt_tr_pre (aa, ab, ac, ad, ae, ba));
-			   RETURN
-			    (False, tl_trailt_tr (aa, ab, ac, ad, ae, ba), c,
-			     (bb, n, xs), e, f,
-			     isa_vmtf_unset (atm_of b)
-			      ((ah, ai, aj, ak, bc), al, bd),
-			     h, fast_minus clvls one_uint32_nat, (am, be), lbd,
-			     outl, (an, ao, ap, aq, ar, bf), (as, at, au, av, bg),
-			     (aw, ax, ay, az, bh), (bi, bj), ra, s, t, u, v, w)
-			 })
-		    xa)
-		\<le> \<Down> (bool_rel \<times>\<^sub>f twl_st_heur_conflict_ana' r)
-		   (RETURN
-		     (let D = resolve_cls_wl' (baa, ca, da, ea, fa, ga, ha) bk bl
-		      in (False, tl baa, ca, Some D, ea, fa, ga, ha))))\<close>
-    if 
-      inv: \<open>update_confl_tl_wl_pre ((bk, bl), baa, ca, da, ea, fa, ga, ha)\<close> and
-      rel: \<open>(((a, b), (aa, ab, ac, ad, ae, ba), c, (af, ag, bb), e, f,
-	 ((ah, ai, aj, ak, bc), al, bd), h, i, (am, be), k, l,
-	 (an, ao, ap, aq, ar, bf), (as, at, au, av, bg), (aw, ax, ay, az, bh),
-	 (bi, bj), ra, s, t, u, v, w),
-	(bk, bl), baa, ca, da, ea, fa, ga, ha)
-       \<in> nat_rel \<times>\<^sub>f nat_lit_lit_rel \<times>\<^sub>f twl_st_heur_conflict_ana' r\<close> and
-      CLS: \<open>CLS = ((bk, bl), baa, ca, da, ea, fa, ga, ha)\<close> and
-      \<open>CLS' =
-       ((a, b), (aa, ab, ac, ad, ae, ba), c, (af, ag, bb), e, f,
-	((ah, ai, aj, ak, bc), al, bd), h, i, (am, be), k, l,
-	(an, ao, ap, aq, ar, bf), (as, at, au, av, bg), (aw, ax, ay, az, bh),
-	(bi, bj), ra, s, t, u, v, w)\<close> and
-      \<open>1 \<le> i\<close> and
-      \<open>lookup_conflict_remove1 b (ag, bb) = (x1, x2)\<close> and
-      pre: \<open>curry6 isa_set_lookup_conflict_aa_pre
-	(aa, ab, ac, ad, ae, ba) c a (af, x1, x2) i k l\<close>
-    for a b aa ab ac ad ae ba c af ag bb e f ah ai aj ak bc al bd h i am be k l an
-       ao ap aq ar bf as at au av bg aw ax ay az bh bi bj ra s t u v w bk bl baa
-       ca da ea fa ga ha x1 x2
-  proof -
-
-    let ?\<A> = \<open>all_atms_st (baa, ca, da, ea, fa, ga, ha)\<close>
-    have
-      ao: \<open>bk \<in># dom_m (get_clauses_wl (baa, ca, da, ea, fa, ga, ha))\<close> and
-      conf: \<open>get_conflict_wl (baa, ca, da, ea, fa, ga, ha) \<noteq> None\<close> and
-      nempty: \<open>get_trail_wl (baa, ca, da, ea, fa, ga, ha) \<noteq> []\<close> and
-      uL_D: \<open>- bl \<in># the (get_conflict_wl (baa, ca, da, ea, fa, ga, ha))\<close> and
-      L_M: \<open>(bl, bk) =
-       lit_and_ann_of_propagated
-	(hd (get_trail_wl (baa, ca, da, ea, fa, ga, ha)))\<close> and
-      bg_D0: \<open>bl \<in># \<L>\<^sub>a\<^sub>l\<^sub>l (?\<A>)\<close> and
-      proped: \<open>is_proped (hd (get_trail_wl (baa, ca, da, ea, fa, ga, ha)))\<close> and
-      \<open>0 < bk\<close> and
-      card_max_lvl: \<open>1 \<le> card_max_lvl (get_trail_wl (baa, ca, da, ea, fa, ga, ha))
-	    (the (get_conflict_wl (baa, ca, da, ea, fa, ga, ha)))\<close> and
-      dist_D: \<open>distinct_mset (the (get_conflict_wl (baa, ca, da, ea, fa, ga, ha)))\<close> and
-      uL_NC: \<open>- bl \<notin> set (get_clauses_wl (baa, ca, da, ea, fa, ga, ha) \<propto> bk)\<close> and
-      L_NC: \<open>2 < length (get_clauses_wl (baa, ca, da, ea, fa, ga, ha) \<propto> bk) \<longrightarrow>
-       bl \<notin> set (tl (get_clauses_wl (baa, ca, da, ea, fa, ga, ha) \<propto> bk))\<close> and
-      L_watch: \<open>bl \<in> set (watched_l
-		  (get_clauses_wl (baa, ca, da, ea, fa, ga, ha) \<propto> bk))\<close> and
-      dist_NC: \<open>distinct (get_clauses_wl (baa, ca, da, ea, fa, ga, ha) \<propto> bk)\<close> and
-      tauto_D: \<open>\<not> tautology (the (get_conflict_wl (baa, ca, da, ea, fa, ga, ha)))\<close> and
-      tauto_NC: \<open>\<not> tautology (mset (get_clauses_wl (baa, ca, da, ea, fa, ga, ha) \<propto> bk))\<close> and
-      tauto_NC_D: \<open>\<not> tautology
-	  (remove1_mset bl
-	    (remove1_mset (- bl) (the (get_conflict_wl (baa, ca, da, ea, fa, ga, ha)) \<union>#
-	     mset (get_clauses_wl (baa, ca, da, ea, fa, ga, ha) \<propto> bk))))\<close> and
-      count_dec_ge: \<open>0 < count_decided (get_trail_wl (baa, ca, da, ea, fa, ga, ha))\<close> and
-      lits: \<open>literals_are_in_\<L>\<^sub>i\<^sub>n (?\<A>)
-	(the (get_conflict_wl (baa, ca, da, ea, fa, ga, ha)))\<close> and
-      lits_confl: \<open>literals_are_\<L>\<^sub>i\<^sub>n (?\<A>)
-	(baa, ca, da, ea, fa, ga, ha)\<close> and
-      lits_trail: \<open>literals_are_in_\<L>\<^sub>i\<^sub>n_trail (?\<A>)
-	(get_trail_wl (baa, ca, da, ea, fa, ga, ha))\<close> 
-      using inv unfolding CLS update_confl_tl_wl_pre_def prod.case apply -
-      by blast+
-
-    have
-      n_d: \<open>no_dup baa\<close> and
-      outl: \<open>out_learned baa da l\<close> and
-      i: \<open>i \<in> counts_maximum_level baa da\<close>
-      using rel unfolding twl_st_heur_conflict_ana_def
-      by auto
-    have
-      [simp]: \<open>a = bk\<close> and
-      [simp]: \<open>b = bl\<close> and
-      n_d: \<open>no_dup baa\<close> and
-      arena: \<open>valid_arena c ca (set ra)\<close> and
-      ocr: \<open>((af, ag, bb), da) \<in> option_lookup_clause_rel ?\<A>\<close> and
-      trail: \<open>((aa, ab, ac, ad, ae, ba), baa) \<in> trail_pol ?\<A>\<close> and
-      bounded: \<open>isasat_input_bounded ?\<A>\<close>
-      using rel by (auto simp: CLS twl_st_heur_conflict_ana_def all_atms_def[symmetric])
-
-    have [simp]: \<open>lit_of (hd baa) = bl\<close> and hd_M_L_C: \<open>hd baa = Propagated bl bk\<close>
-      using L_M nempty proped by (cases baa; cases \<open>hd baa\<close>; auto; fail)+
-
-    have bg_D[simp]: \<open>bl \<notin># the da\<close>
-      using uL_D tauto_D by (auto simp: tautology_add_mset add_mset_eq_add_mset
-      dest!: multi_member_split)
-    have bg_\<A>: \<open>bl \<in># \<L>\<^sub>a\<^sub>l\<^sub>l ?\<A>\<close>
-      using  \<open>lit_of (hd baa) = bl\<close> lits_trail uL_D nempty
-      by (cases baa)
-        (auto simp del: \<open>lit_of (hd baa) = bl\<close> simp: literals_are_in_\<L>\<^sub>i\<^sub>n_trail_Cons)
-
-    have [simp]: \<open>length (ca \<propto> bk) > 2 \<Longrightarrow> bl \<notin> set (tl (ca \<propto> bk))\<close>
-      using L_NC
-      by (auto simp: resolve_cls_wl'_def split: if_splits)
-    have mset_ge0_iff:  "0 < size M \<longleftrightarrow> M \<noteq> {#}" for M
-     by (cases M) auto
-    have no_dup: \<open>L \<in> set ((ca \<propto> bk)) \<Longrightarrow>
-       - L \<in># remove1_mset (-bl) (the da) \<Longrightarrow> False\<close> for L
-      using tauto_NC_D tauto_NC \<open>length (ca \<propto> bk) > 2 \<Longrightarrow> bl \<notin> set (tl (ca \<propto> bk))\<close> uL_NC
-        tauto_D uL_D dist_D L_watch dist_NC
-      apply (cases \<open>- L \<in># mset (ca \<propto> bk)\<close>; cases \<open>bl = L\<close>)
-      apply (auto dest!: multi_member_split
-        simp: sup_union_left2 add_mset_remove_trivial_If tautology_add_mset in_set_tlD
-          add_mset_eq_add_mset
-        split: if_splits)
-      apply (cases \<open>ca \<propto> bk\<close>;
-        cases \<open>tl (ca \<propto> bk)\<close>)
-	apply (auto simp: tautology_add_mset)
-      done
-
-    have size_union_ge1: \<open>Suc 0 \<le> size A \<Longrightarrow> Suc 0 \<le> size (A \<union># B)\<close> for A B
-      apply (cases A)
-      apply (simp; fail)
-      apply (case_tac \<open>x \<in># B\<close>)
-      by (auto dest!: multi_member_split simp: add_mset_union)
-
-    let ?da = \<open>Some (remove1_mset (-bl) (the da))\<close>
-    have merge_conflict_m_pre: \<open>merge_conflict_m_pre ?\<A> ((((((baa, ca), bk), ?da), i), k), l)\<close>
-      using rel conf dist_D dist_NC tauto_NC n_d outl i lits lits_confl bounded ao no_dup
-      multi_member_split[OF uL_D]
-      (*no_dup*)
-      unfolding merge_conflict_m_pre_def counts_maximum_level_def literals_are_\<L>\<^sub>i\<^sub>n_def
-      is_\<L>\<^sub>a\<^sub>l\<^sub>l_def literals_are_in_\<L>\<^sub>i\<^sub>n_mm_def
-      apply (auto simp: all_lits_of_mm_union all_lits_def literals_are_in_\<L>\<^sub>i\<^sub>n_add_mset)
-      
-      oops
-      using ao conf dist_D dist_NC tauto_NC n_d outl i no_dup lits lits_confl bounded
-      unfolding merge_conflict_m_pre_def counts_maximum_level_def literals_are_\<L>\<^sub>i\<^sub>n_def
-      is_\<L>\<^sub>a\<^sub>l\<^sub>l_def literals_are_in_\<L>\<^sub>i\<^sub>n_mm_def
-      by (auto simp: all_lits_of_mm_union all_lits_def)
-
-    have ?thesis
-       using rel inv
-       apply -
-       apply (rule order_trans)
-       apply (rule isa_resolve_merge_conflict[of ?\<A> \<open>set ra\<close>,
-         THEN fref_to_Down_curry6, OF _])
-       subgoal using arena ocr trail by (auto simp: all_atms_def[symmetric])
-       subgoal unfolding merge_conflict_m_def conc_fun_SPEC
-        by (auto simp: twl_st_heur_conflict_ana_def merge_conflict_m_def update_confl_tl_wl_pre_def
-           resolve_cls_wl'_def ac_simps no_dup_tlD lookup_remove1_uminus arena_in_L
-	   all_atms_def[symmetric]
-           intro!: ASSERT_refine_left
-	     tl_trail_tr[THEN fref_to_Down_unRET])
-    have lookup_remove1_uminus:
-       \<open>lookup_conflict_remove1 (-bg) A = lookup_conflict_remove1 bg A\<close> for A
-      by (auto simp: lookup_conflict_remove1_def)
-    have [simp]: \<open>lit_of (hd baa) = bg\<close> and hd_M_L_C: \<open>hd baa = Propagated bg ao\<close>
-      using L_M nempty proped by (cases baa; cases \<open>hd baa\<close>; auto; fail)+
-    have bg_D[simp]: \<open>bg \<notin># the da\<close>
-      using uL_D tauto_D by (auto simp: tautology_add_mset add_mset_eq_add_mset
-      dest!: multi_member_split)
-    have bg_\<A>: \<open>bg \<in># \<L>\<^sub>a\<^sub>l\<^sub>l ?\<A>\<close>
-      using  \<open>lit_of (hd baa) = bg\<close> lits_trail uL_D nempty
-      by (cases baa)
-        (auto simp del: \<open>lit_of (hd baa) = bg\<close> simp: literals_are_in_\<L>\<^sub>i\<^sub>n_trail_Cons)
-
-    have [simp]: \<open>length (ca \<propto> ao) > 2 \<Longrightarrow> bg \<notin> set (tl (ca \<propto> ao))\<close>
-      using L_NC
-      by (auto simp: resolve_cls_wl'_def split: if_splits)
-    have mset_ge0_iff:  "0 < size M \<longleftrightarrow> M \<noteq> {#}" for M
-     by (cases M) auto
-    have no_dup: \<open>length (ca \<propto> ao) > 2 \<Longrightarrow> L \<in> set (tl (ca \<propto> ao)) \<Longrightarrow> - L \<in># the da \<Longrightarrow> False\<close> for L
-      using tauto_NC_D tauto_NC \<open>length (ca \<propto> ao) > 2 \<Longrightarrow> bg \<notin> set (tl (ca \<propto> ao))\<close>
-      apply (cases \<open>- L \<in># mset (tl (ca \<propto> ao))\<close>; cases \<open>bg = L\<close>)
-      apply (auto dest!: multi_member_split
-      simp: sup_union_left2 add_mset_remove_trivial_If tautology_add_mset split: if_splits)
-      apply (metis in_set_tlD set_mset_mset tautology_minus)
-      by (metis \<open>bg \<notin># the da\<close> in_remove1_mset_neq insert_DiffM set_mset_mset
-        subset_mset.sup.right_idem subset_mset.sup_commute sup_union_left1 uminus_of_uminus_id
-        union_single_eq_member)
-    have size_union_ge1: \<open>Suc 0 \<le> size A \<Longrightarrow> Suc 0 \<le> size (A \<union># B)\<close> for A B
-      apply (cases A)
-      apply (simp; fail)
-      apply (case_tac \<open>x \<in># B\<close>)
-      by (auto dest!: multi_member_split simp: add_mset_union)
-    have merge_conflict_m_pre: \<open>merge_conflict_m_pre ?\<A> ((((((baa, ca), ao), da), i), k), ag)\<close>
-      using ao conf dist_D dist_NC tauto_NC n_d outl i no_dup lits lits_confl bounded
-      unfolding merge_conflict_m_pre_def counts_maximum_level_def literals_are_\<L>\<^sub>i\<^sub>n_def
-      is_\<L>\<^sub>a\<^sub>l\<^sub>l_def literals_are_in_\<L>\<^sub>i\<^sub>n_mm_def
-      by (auto simp: all_lits_of_mm_union all_lits_def)
-
-    have arena_in_L: \<open>arena_lit c C \<in># \<L>\<^sub>a\<^sub>l\<^sub>l ?\<A>\<close>
-      if \<open>Suc ao \<le> C\<close> \<open>C < ao + arena_length c ao\<close> for C
-    proof -
-      define D where \<open>D = C - ao\<close>
-      with that have [simp]: \<open>C = ao + D\<close> and D_le: \<open>D < arena_length c ao\<close>
-        by auto
-
-      have is_in: \<open>ca \<propto> ao ! D \<in># mset (ca \<propto> ao)\<close>
-        using arena that D_le ao
-        by (auto intro!: nth_mem simp: arena_lifting(4))
-      have \<open>set_mset (all_lits_of_m (mset (ca \<propto> ao))) \<subseteq> set_mset (\<L>\<^sub>a\<^sub>l\<^sub>l ?\<A>)\<close>
-        using lits ao by (auto simp: literals_are_\<L>\<^sub>i\<^sub>n_def ran_m_def all_lits_of_mm_add_mset
-          is_\<L>\<^sub>a\<^sub>l\<^sub>l_def all_lits_def
-        dest!: multi_member_split)
-      then have \<open>ca \<propto> ao ! D \<in># \<L>\<^sub>a\<^sub>l\<^sub>l ?\<A>\<close>
-        using multi_member_split[OF is_in]
-        by (auto simp: all_lits_of_m_add_mset)
-
-      then show ?thesis
-        using arena ao D_le by (auto simp: arena_lifting)
-    qed
-
-    have [simp]: \<open>- bg \<notin># remove1_mset (- bg) (the da)\<close>
-      using dist_D uL_D multi_member_split[of \<open>-bg\<close> \<open>the da\<close>]
-      by auto
-    moreover have [simp]: \<open>- bg \<notin> set (tl (ca \<propto> ao))\<close>
-      using uL_D proped L_M nempty uL_NC
-      by (cases \<open>ca \<propto> ao\<close>) (auto simp: resolve_cls_wl'_def split: if_splits)
-    ultimately have [simp]: \<open>- bg \<notin># remove1_mset (- bg) (the da \<union># mset (tl (ca \<propto> ao)))\<close>
-      by (metis \<open>a = ao\<close> diff_single_trivial in_multiset_in_set multi_drop_mem_not_eq
-            remove1_mset_union_distrib)
-
-    have \<open>vmtf_unset_pre (atm_of b) ivmtf\<close>
-      if \<open>ivmtf \<in> isa_vmtf ?\<A> baa\<close>
-      apply (rule vmtf_unset_pre'[OF that])
-      using  that bg_\<A>
-      by (auto simp: vmtf_unset_pre_def in_\<L>\<^sub>a\<^sub>l\<^sub>l_atm_of_\<A>\<^sub>i\<^sub>n)
-    moreover have \<open>isa_vmtf_unset (atm_of bg) ivmtf \<in> isa_vmtf ?\<A> (tl baa)\<close>
-      if \<open>ivmtf \<in> isa_vmtf ?\<A> baa\<close>
-      by (rule isa_vmtf_tl_isa_vmtf[OF that])
-        (use inv rel that in \<open>auto simp: atms_of_def update_confl_tl_wl_pre_def
-          twl_st_heur_conflict_ana_def
-        intro!: isa_vmtf_unset_isa_vmtf\<close>)
-    moreover have
-      \<open>out_learned (tl baa) (Some (remove1_mset (- bg) ((the da) \<union># mset (tl (ca \<propto> ao))))) b\<close>
-      if H: \<open>out_learned baa (Some ((the da) \<union># mset (tl (ca \<propto> ao)))) b\<close> for b
-    proof -
-      have \<open>(- bg) \<notin># {#bg \<in># (the da). get_level baa bg < count_decided baa#}\<close>
-        using L_M nempty proped
-        by (cases baa; cases \<open>hd baa\<close>) auto
-      then have out:
-        \<open>out_learned baa (Some (resolve_cls_wl' (baa, ca, Some (the da), ea, fa, ga, ha) ao bg)) b\<close>
-        using uL_D H
-        by (auto simp: resolve_cls_wl'_def out_learned_def ac_simps)
-      have \<open>out_learned (tl baa)
-        (Some (resolve_cls_wl' (baa, ca, Some (the da), ea, fa, ga, ha) ao bg)) b\<close>
-        apply (rule out_learned_tl_Some_notin[THEN iffD1])
-        using uL_D out proped L_M nempty proped nempty
-        by (cases baa; cases \<open>hd baa\<close>; auto simp: resolve_cls_wl'_def split: if_splits; fail)+
-    then show ?thesis
-      using rel
-      by (auto simp: twl_st_heur_conflict_ana_def merge_conflict_m_def update_confl_tl_wl_pre_def
-          resolve_cls_wl'_def ac_simps)
-    qed
-    moreover have \<open>card_max_lvl baa (mset (tl (ca \<propto> ao)) \<union># (the da)) - Suc 0
-      \<in> counts_maximum_level (tl baa)
-        (Some (resolve_cls_wl' (baa, ca, da, ea, fa, ga, ha) ao bg))\<close>
-    proof -
-      have \<open>distinct_mset (remove1_mset (- bg) (the da \<union># mset (tl (ca \<propto> ao))))\<close>
-        using dist_NC dist_D by (auto intro!: distinct_mset_minus)
-      moreover have \<open>\<not>tautology (remove1_mset (- bg) (the da \<union># mset (tl (ca \<propto> ao))))\<close>
-        using tauto_NC_D by simp
-      moreover have \<open>card_max_lvl baa (mset (tl (ca \<propto> ao)) \<union># the da) - 1 =
-        card_max_lvl baa (remove1_mset (- bg) (the da \<union># mset (tl (ca \<propto> ao))))\<close>
-        unfolding \<open>lit_of (hd baa) = bg\<close> [symmetric]
-        apply (subst card_max_lvl_remove1_mset_hd)
-        using uL_D
-        by (auto simp: hd_M_L_C ac_simps)
-      ultimately show ?thesis
-        unfolding counts_maximum_level_def
-        using uL_D L_M proped nempty \<open>ao > 0\<close> n_d count_dec_ge
-        by (auto simp del: simp: card_max_lvl_tl resolve_cls_wl'_def card_max_lvl_remove1_mset_hd)
-    qed
-    moreover have \<open>da = Some y \<Longrightarrow> ((a, aaa, b), Some (y \<union># mset (tl (ca \<propto> ao))))
-       \<in> option_lookup_clause_rel ?\<A> \<Longrightarrow>
-       ((a, lookup_conflict_remove1 (-bg) (aaa, b)),
-        Some (remove1_mset (- bg) (y \<union># mset (tl (ca \<propto> ao)))))
-       \<in> option_lookup_clause_rel ?\<A>\<close>
-       for a aaa b ba y
-       using uL_D bg_D0 bg_D
-       using lookup_conflict_remove1[THEN fref_to_Down_unRET_uncurry, of ?\<A> \<open>-bg\<close>
-          \<open>y \<union># mset (tl (ca \<propto> ao))\<close> \<open>-bg\<close> \<open>(aaa, b)\<close>]
-       by (auto simp: option_lookup_clause_rel_def
-         size_remove1_mset_If image_image uminus_\<A>\<^sub>i\<^sub>n_iff)
-    moreover have \<open>1 \<le> card_max_lvl baa (the da \<union># mset (tl (ca \<propto> ao)))\<close>
-      using card_max_lvl by (auto simp: card_max_lvl_def size_union_ge1)
-    moreover have \<open>((a, aaa, b), Some (the da \<union># mset (tl (ca \<propto> ao))))
-       \<in> option_lookup_clause_rel ?\<A> \<Longrightarrow>
-       lookup_conflict_remove1_pre (bg, aaa, b)\<close>
-       for a aaa b ba y
-       using uL_D bg_D0 bg_D uL_D
-       by (auto simp: option_lookup_clause_rel_def lookup_clause_rel_def atms_of_def
-         lookup_conflict_remove1_pre_def mset_ge0_iff
-         size_remove1_mset_If image_image uminus_\<A>\<^sub>i\<^sub>n_iff simp del: bg_D)
-    moreover have \<open>tl_trailt_tr_pre ba\<close>
-      by (rule tl_trailt_tr_pre[OF _ trail])
-        (use nempty in auto)
-    ultimately show ?thesis
-       using rel inv
-       apply -
-       apply (rule order_trans)
-       apply (rule isa_resolve_merge_conflict[of ?\<A> \<open>set an\<close>,
-         THEN fref_to_Down_curry6, OF merge_conflict_m_pre])
-       subgoal using arena ocr trail by (auto simp: all_atms_def[symmetric])
-       subgoal unfolding merge_conflict_m_def conc_fun_SPEC
-        by (auto simp: twl_st_heur_conflict_ana_def merge_conflict_m_def update_confl_tl_wl_pre_def
-           resolve_cls_wl'_def ac_simps no_dup_tlD lookup_remove1_uminus arena_in_L
-	   all_atms_def[symmetric]
-           intro!: ASSERT_refine_left
-	     tl_trail_tr[THEN fref_to_Down_unRET])
-       done  
-    show ?thesis sorry
-  qed
-*)
 
   have isasat_lookup_merge_eq2:
     \<open>isasat_lookup_merge_eq2 b (aa, ab, ac, ad, ae, ba) c a (af, ag, bb) i k l
@@ -969,7 +684,7 @@ proof -
       le2: \<open>arena_length c a = 2\<close>
     for a b aa ab ac ad ae ba c af ag bb e f ah ai aj ak bc al bd h i am be k l an
 	 ao ap aq ar bf as at au av bg aw ax ay az bh bi bj ra s t u v w bk bl baa
-	 ca da ea fa ga ha
+	 ca da ea fa ga ha CLS CLS'
   proof -
     let ?\<A> = \<open>all_atms_st (baa, ca, da, ea, fa, ga, ha)\<close>
     have
@@ -1218,7 +933,8 @@ proof -
 
   have isa_set_lookup_conflict_aa_pre:
     \<open>curry6 isa_set_lookup_conflict_aa_pre
-	 (aa, ab, ac, ad, ae, ba) c a (af, ag, bb) i k l\<close>
+	 (aa, ab, ac, ad, ae, ba) c a (af, ag, bb) i k l\<close> (is ?A) and
+    valid: \<open>arena_is_valid_clause_idx c a\<close> (is ?B)
     if 
       inv: \<open>update_confl_tl_wl_pre ((bk, bl), baa, ca, da, ea, fa, ga, ha)\<close> and
       \<open>1 \<le> i\<close> and
@@ -1253,10 +969,14 @@ proof -
       trail: \<open>((aa, ab, ac, ad, ae, ba), baa) \<in> trail_pol ?\<A>\<close> and
       [simp]: \<open>bk = a\<close>
       using rel by (auto simp: CLS twl_st_heur_conflict_ana_def all_atms_def[symmetric])
-    show ?thesis
+    show ?A
       using arena lits_trail ao
       unfolding isa_set_lookup_conflict_aa_pre_def
       by (auto simp: arena_lifting lookup_conflict_remove1_def)
+    show ?B
+      using arena ao
+      unfolding arena_is_valid_clause_idx_def
+      by auto
   qed
   show ?thesis
     supply [[goals_limit = 2]]
@@ -1273,14 +993,9 @@ proof -
             RES_RETURN_RES RETURN_def counts_maximum_level_def)
       subgoal
         by (rule isa_set_lookup_conflict_aa_pre)
-      subgoal for a b aa ab ac ad ae ba c af ag bb e f ah ai aj ak bc al bd h i am be k l an
-       ao ap aq ar bf as at au av bg aw ax ay az bh bi bj ra s t u v w bk bl baa
-       ca da ea fa ga ha
-       explore_have
-      
-      by (rule H)
-      subgoal
-      sorry
+      subgoal by (rule valid)
+      subgoal by (rule isasat_lookup_merge_eq2)
+      subgoal by (rule H)
       done
     done
 qed
@@ -2002,28 +1717,6 @@ declare
   tl_state_wl_heur_code.refine[sepref_fr_rules]
   tl_state_wl_heur_fast_code.refine[sepref_fr_rules]
 
-(*
-lemma option_lookup_clause_assn_the[sepref_fr_rules]:
-  \<open>(return o snd, RETURN o the) \<in> [\<lambda>C. C \<noteq> None]\<^sub>a option_lookup_clause_assn\<^sup>d \<rightarrow> lookup_clause_assn\<close>
-  by sepref_to_hoare
-    (sep_auto simp: lookup_clause_assn_def option_lookup_clause_assn_def lookup_clause_rel_def
-       hr_comp_def option_lookup_clause_rel_def)
-
-lemma option_lookup_clause_assn_Some[sepref_fr_rules]:
-  \<open>(return o (\<lambda>C. (False, C)), RETURN o Some) \<in> lookup_clause_assn\<^sup>d \<rightarrow>\<^sub>a option_lookup_clause_assn\<close>
-  by sepref_to_hoare
-    (sep_auto simp: lookup_clause_assn_def option_lookup_clause_assn_def lookup_clause_rel_def
-       hr_comp_def option_lookup_clause_rel_def bool_assn_alt_def)
-
-lemma lookup_clause_assn_op_nset_is_emty[sepref_fr_rules]:
-  \<open>(return o (\<lambda>(n, _). n = 0), RETURN o op_mset_is_empty) \<in> lookup_clause_assn\<^sup>k \<rightarrow>\<^sub>a bool_assn\<close>
-  apply sepref_to_hoare
-  apply (rename_tac x xi, case_tac xi)
-  by (sep_auto simp: lookup_clause_assn_def lookup_clause_rel_def hr_comp_def
-    uint32_nat_assn_0_eq uint32_nat_rel_def br_def pure_def nat_of_uint32_0_iff)+
-
-*)
-
 sepref_register update_confl_tl_wl_heur
 sepref_definition update_confl_tl_wl_code
   is \<open>uncurry2 update_confl_tl_wl_heur\<close>
@@ -2033,6 +1726,7 @@ sepref_definition update_confl_tl_wl_code
   supply [[goals_limit=1]]
   unfolding update_confl_tl_wl_heur_def isasat_unbounded_assn_def
     update_confl_tl_wl_heur_pre_def PR_CONST_def
+    two_uint64_nat_def[symmetric]
   by sepref
 
 sepref_definition update_confl_tl_wl_fast_code
